\documentclass[./main]{subfiles}

\begin{document}
(2)
$ ( \tan \theta)' = \frac{1}{\cos^2 \theta} $ より、

\begin{eqnarray}
 ( \tan \theta ・ \frac{1}{\cos^{n-2} \theta}) '
& = & \frac{1}{\cos^n \theta} +  \tan \theta ・  \frac{2-n}{\cos^{n-1} \theta} ・ ( - \sin \theta) \\
& = & \frac{1}{\cos^n \theta} +  \frac{n-2}{\cos^{n} \theta} ・ \sin^2 \theta \\
& = & \frac{1}{\cos^n \theta} +  \frac{n-2}{\cos^{n} \theta} ・ (1 -  \cos^2 \theta ) \\
& = & \frac{1}{\cos^n \theta} +  \frac{n-2}{\cos^{n} \theta} + \frac{n-2}{\cos^{n-2} \theta} \\
& = & \frac{n-1}{\cos^{n} \theta} + \frac{n-2}{\cos^{n-2} \theta} \\
\end{eqnarray}

この式の両辺を０から$\frac{\pi}{3}$ まで積分する。

\begin{eqnarray}
(右辺） 
& = &  \int_{0}^{\frac{\pi}{3}} (\frac{n-1}{\cos^{n} \theta} + \frac{n-2}{\cos^{n-2} \theta} ) d\theta \\
& = & (n-1)I_{n} - (n-2) I_{n-2}
\end{eqnarray}

\begin{eqnarray}
(左辺） 
& = &  \int_{0}^{\frac{\pi}{3}} ( \tan \theta ・ \frac{1}{\cos^{n-2} \theta}) 'd\theta \\
& = &　\sqrt{3}・\frac{1}{(\frac{1}{2})^{n-2}}
\end{eqnarray}

式を整理して、

\begin{equation}
I_{n}=\frac{(n-2)I_{n-2}+\sqrt{3}・2^{n-2}}{n-1}
\end{equation}

\end{document}